Proving total correctness while rule for designs
git-svn-id: orca@469

C-verifier/src/Midend-IVL/Isabelle-UTP-Extended/hoare/HoareLogic/TotalCorrectness/Des/utp_hoare_des.thy
@@ -3,9 +3,169 @@ theory utp_hoare_des
 imports "../../../../utp/utp_rec_total_des"
 
 begin
-
-subsection \<open>Try Catch laws\<close>
-(*see utp_hoare_helper*)
 section {*Hoare logic for designs*}  
+named_theorems hoare_total
+
+subsection {*Hoare triple definition*}
+
+definition hoare_d :: "'\<alpha> cond \<Rightarrow> '\<alpha> hrel_des \<Rightarrow> '\<alpha> cond \<Rightarrow> bool" ("\<lbrace>_\<rbrace>_\<lbrace>_\<rbrace>\<^sub>D") where
+[upred_defs]:"\<lbrace>p\<rbrace>Q\<lbrace>r\<rbrace>\<^sub>D = ((\<lceil>p\<rceil>\<^sub>D\<^sub>< \<turnstile> \<lceil>r\<rceil>\<^sub>D\<^sub>>) \<sqsubseteq> Q)"
+
+lemma hoare_true_assisgns_d_t [hoare_total]: 
+  "\<lbrace>p\<rbrace>\<langle>\<sigma>\<rangle>\<^sub>D\<lbrace>true\<rbrace>\<^sub>D"
+  by rel_auto
+
+lemma hoare_true_skip_d_t [hoare_total]: 
+  "\<lbrace>p\<rbrace>SKIP\<^sub>D\<lbrace>true\<rbrace>\<^sub>D"
+  by rel_auto
+
+lemma hoare_false_d_t [hoare_total]: 
+  "\<lbrace>false\<rbrace>C\<lbrace>q\<rbrace>\<^sub>D"
+  by rel_auto
+
+subsection {*Precondition weakening*}
+
+lemma hoare_pre_weak_d_t[hoare_total]:
+  assumes "`p\<^sub>1 \<Rightarrow> p\<^sub>2`" and "\<lbrace>p\<^sub>2\<rbrace>C\<lbrace>q\<rbrace>\<^sub>D"
+  shows "\<lbrace>p\<^sub>1\<rbrace>C\<lbrace>q\<rbrace>\<^sub>D" 
+  by (insert assms) rel_auto
+
+subsection {*Post-condition strengthening*}
+
+lemma hoare_post_weak_d_t[hoare_total]:
+  assumes "\<lbrace>p\<rbrace>C\<lbrace>q\<^sub>2\<rbrace>\<^sub>D" and "`q\<^sub>2 \<Rightarrow> q\<^sub>1`"
+  shows "\<lbrace>p\<rbrace>C\<lbrace>q\<^sub>1\<rbrace>\<^sub>D" 
+ by (insert assms) rel_auto
+
+subsection {*Hoare and assertion logic*}
+
+lemma hoare_r_conj_d_t [hoare_total]: 
+  assumes"\<lbrace>p\<rbrace>C\<lbrace>r\<rbrace>\<^sub>D" and "\<lbrace>p\<rbrace>C\<lbrace>s\<rbrace>\<^sub>D"
+  shows "\<lbrace>p\<rbrace>C\<lbrace>r \<and> s\<rbrace>\<^sub>D"
+  by (insert assms) rel_auto
+
+subsection {*Hoare SKIP*}
+
+lemma skip_d_hoare_d_t [hoare_total]: 
+  "\<lbrace>p\<rbrace>SKIP\<^sub>D\<lbrace>p\<rbrace>\<^sub>D"
+  by rel_auto
+
+subsection {*Hoare for assignment*}
+
+lemma assigns_d_hoare_d_t [hoare_total]: 
+  assumes"`p \<Rightarrow> \<sigma> \<dagger> q`" 
+  shows  "\<lbrace>p\<rbrace>\<langle>\<sigma>\<rangle>\<^sub>D\<lbrace>q\<rbrace>\<^sub>D"
+  by (insert assms) rel_auto
+
+lemma assigns_d_hoare_d'_t [hoare_total]: 
+  "\<lbrace>\<sigma> \<dagger> p\<rbrace>\<langle>\<sigma>\<rangle>\<^sub>D\<lbrace>p\<rbrace>\<^sub>D"
+  by rel_auto
+
+lemma assigns_d_floyd_d_t [hoare_total]:
+  assumes \<open>vwb_lens x\<close>
+  shows \<open>\<lbrace>p\<rbrace>x :=\<^sub>D e\<lbrace>\<^bold>\<exists>v \<bullet> p\<lbrakk>\<guillemotleft>v\<guillemotright>/x\<rbrakk> \<and> &x =\<^sub>u e\<lbrakk>\<guillemotleft>v\<guillemotright>/x\<rbrakk>\<rbrace>\<^sub>D\<close>
+  apply (insert assms)
+  apply rel_simp
+  apply transfer
+  apply (rule_tac x = \<open>get\<^bsub>x\<^esub> more\<close> in exI)
+  apply auto
+  done
+
+subsection {*Hoare for Sequential Composition*}
+
+lemma seq_hoare_d_t [hoare_total]: 
+  assumes"\<lbrace>p\<rbrace>C\<^sub>1\<lbrace>s\<rbrace>\<^sub>D" and "\<lbrace>s\<rbrace>C\<^sub>2\<lbrace>r\<rbrace>\<^sub>D" 
+  shows"\<lbrace>p\<rbrace>C\<^sub>1 ;; C\<^sub>2\<lbrace>r\<rbrace>\<^sub>D"
+  by (insert assms, rel_auto) metis+ 
+
+subsection {*Hoare for Conditional*}
+
+lemma cond_d_hoare_d_t [hoare_total]: 
+  assumes "\<lbrace>b \<and> p\<rbrace>C\<^sub>1\<lbrace>q\<rbrace>\<^sub>D" and "\<lbrace>\<not>b \<and> p\<rbrace>C\<^sub>2\<lbrace>q\<rbrace>\<^sub>D" 
+  shows "\<lbrace>p\<rbrace>C\<^sub>1 \<triangleleft> \<lceil>b\<rceil>\<^sub>D\<^sub>< \<triangleright> C\<^sub>2\<lbrace>q\<rbrace>\<^sub>D"
+  by (insert assms, rel_auto) metis+ 
+
+lemma cond_d_hoare_d'_t [hoare_total]: 
+  assumes "\<lbrace>p\<rbrace>\<lceil>b\<rceil>\<^sub>D\<^sub>< \<and> C\<^sub>1\<lbrace>q\<rbrace>\<^sub>D" and "\<lbrace>p\<rbrace>\<lceil>\<not>b\<rceil>\<^sub>D\<^sub>< \<and> C\<^sub>2\<lbrace>q\<rbrace>\<^sub>D" 
+  shows "\<lbrace>p\<rbrace>bif\<^sub>D b then C\<^sub>1 else C\<^sub>2 eif \<lbrace>q\<rbrace>\<^sub>D"
+  by (insert assms, rel_auto) 
+
+subsection {*Hoare for While-loop*}
+term " x:=\<^sub>D s"  
+term "while b do x:=\<^sub>D s od"
+term "(\<lceil>b \<and> I \<and>  E =\<^sub>u \<guillemotleft>st\<guillemotright> \<rceil>\<^sub>< \<Rightarrow> (\<lceil>I \<and>(E,\<guillemotleft>st\<guillemotright>)\<^sub>u\<in>\<^sub>u\<guillemotleft>R\<guillemotright> \<rceil>\<^sub>> )) \<sqsubseteq> (P \<turnstile> Q)"  
+  
+lemma cond_refine_des: 
+  assumes "((b \<and> p) \<turnstile> q) \<sqsubseteq> C\<^sub>1" and "((\<not>b \<and> p) \<turnstile> q)\<sqsubseteq> C\<^sub>2" 
+  shows "(p \<turnstile> q) \<sqsubseteq> (C\<^sub>1 \<triangleleft> b \<triangleright> C\<^sub>2)"
+  using assms by rel_blast
+thm seq_refine_unrest
+    
+lemma seq_refine_unrest_des:
+  assumes "$ok\<acute> \<sharp> P\<^sub>1" "$ok\<acute> \<sharp> P\<^sub>2" 
+           "out\<alpha> \<sharp> Q\<^sub>1" "out\<alpha> \<sharp> p" "in\<alpha> \<sharp> q"
+  assumes "(p \<turnstile> \<lceil>s\<rceil>\<^sub>D\<^sub>>) \<sqsubseteq> (P\<^sub>1 \<turnstile> Q\<^sub>1)" and "(\<lceil>s\<rceil>\<^sub>D\<^sub>> \<turnstile> q) \<sqsubseteq> (P\<^sub>2 \<turnstile> Q\<^sub>2)"
+  shows "(p \<turnstile> q) \<sqsubseteq> ((P\<^sub>1 \<turnstile> Q\<^sub>1) ;; (P\<^sub>2 \<turnstile> Q\<^sub>2))"
+  using assms apply pred_simp apply rel_auto
+  apply metis+ done 
+   
+lemma while_hoare_r_t [hoare_total]:
+  assumes WF: "wf R"
+  assumes I0: "`Pre \<Rightarrow> I`"  
+  assumes induct_step:"\<And> st. (\<lceil>b \<and> I \<and>  E =\<^sub>u \<guillemotleft>st\<guillemotright> \<rceil>\<^sub>D\<^sub>< \<turnstile> (\<lceil>I \<and>(E,\<guillemotleft>st\<guillemotright>)\<^sub>u\<in>\<^sub>u\<guillemotleft>R\<guillemotright> \<rceil>\<^sub>D\<^sub>> )) \<sqsubseteq> (\<lceil>P\<rceil>\<^sub>D \<turnstile> \<lceil>Q\<rceil>\<^sub>D)"  
+  assumes PHI:"`(\<not> \<lceil>b\<rceil>\<^sub>D\<^sub>< \<and> \<lceil>I\<rceil>\<^sub>D\<^sub><) \<turnstile> \<lceil>Post\<rceil>\<^sub>D\<^sub>>`"  
+  shows "\<lbrace>Pre\<rbrace>while  b invr I do \<lceil>P\<rceil>\<^sub>D \<turnstile> \<lceil>Q\<rceil>\<^sub>D od\<lbrace>\<not>Post \<and> p\<rbrace>\<^sub>D"
+proof -
+  have M: "mono (\<lambda>X. bif\<^sub>D b then ((\<lceil>P\<rceil>\<^sub>D \<turnstile> \<lceil>Q\<rceil>\<^sub>D) ;; X) else SKIP\<^sub>D eif)"
+    by (auto intro: monoI seqr_mono cond_mono) 
+   have H: "(\<lambda>X. bif\<^sub>D b then ((\<lceil>P\<rceil>\<^sub>D \<turnstile> \<lceil>Q\<rceil>\<^sub>D) ;; X) else SKIP\<^sub>D eif) \<in> \<lbrakk>\<^bold>H\<rbrakk>\<^sub>H \<rightarrow> \<lbrakk>\<^bold>H\<rbrakk>\<^sub>H" 
+    apply pred_simp apply rel_simp apply smt done   
+  from mono_Monotone_utp_order [OF M, of "\<H>\<^bsub>DES\<^esub>"] H
+          design_theory_continuous.LFP_weak_unfold  
+  have M_des: "Mono\<^bsub>uthy_order DES\<^esub>(\<lambda>X. bif\<^sub>D b then (\<lceil>P\<rceil>\<^sub>D \<turnstile> \<lceil>Q\<rceil>\<^sub>D) ;; X else SKIP\<^sub>D eif)"
+    by auto
+  show ?thesis    
+  unfolding  hoare_d_def While_inv_des_def While_lfp_des_def
+   apply (rule hoare_pre_weak_d_t[unfolded hoare_d_def ,of _ "I" ])
+  using I0 
+   apply pred_simp
+    apply (rule rec_total_utp_des_rule[where Pre="\<lceil>I\<rceil>\<^sub>D\<^sub><" and E = "E", OF WF ])  
+      apply (simp add: M_des)
+     apply (simp add: H)
+    apply pred_simp
+   apply pred_simp
+  apply (rule  cond_refine_des)
+    subgoal for  st
+      apply (rule_tac seq_refine_unrest_des[where s= "I \<and> (E,\<guillemotleft>st\<guillemotright>)\<^sub>u\<in>\<^sub>u\<guillemotleft>R\<guillemotright>" ])
+            apply pred_simp
+           apply pred_simp
+         
+        apply pred_simp
+  apply (rule   seq_hoare_d_t[unfolded hoare_d_def])
+    thm cond_d_hoare_d_t[unfolded hoare_d_def]
+     prefer 2
+   apply (rule skip_refine_rel)
+  using PHI
+   apply pred_blast
+    subgoal for  st 
+      apply (rule_tac seq_refine_unrest[where s= "I \<and> (E,\<guillemotleft>st\<guillemotright>)\<^sub>u\<in>\<^sub>u\<guillemotleft>R\<guillemotright>" ])
+         apply pred_simp
+        apply pred_simp
+       apply (rule order_trans[OF induct_step, where st1 = st]) 
+       apply pred_simp 
+      apply pred_simp
+done        
+  done 
+
+lemma while_hoare_r'_t [hoare_total]:
+  assumes "\<lbrace>p \<and> b\<rbrace>C\<lbrace>p\<rbrace>\<^sub>A\<^sub>B\<^sub>R" and "`p \<and> \<not>b \<Rightarrow> q`"
+  shows "\<lbrace>p\<rbrace>while b do C od\<lbrace>q\<rbrace>\<^sub>A\<^sub>B\<^sub>R"
+  using assms
+  by (metis hoare_post_weak_t while_hoare_r_t inf_commute)
+
+lemma while_invr_hoare_r_t [hoare_total]:
+  assumes "\<lbrace>p \<and> b\<rbrace>C\<lbrace>p\<rbrace>\<^sub>A\<^sub>B\<^sub>R" and "`pre \<Rightarrow> p`" and "`(\<not>b \<and> p) \<Rightarrow> post`"
+  shows "\<lbrace>pre\<rbrace>while b invr p do C od\<lbrace>post\<rbrace>\<^sub>A\<^sub>B\<^sub>R"
+  by (metis assms hoare_pre_str_t while_hoare_r'_t While_inv_def inf_commute)
   
 end
